Test_Tmp_Hoare.thy
@@ -124,13 +124,18 @@ lemma True proof
   (* TODO should work *)
   (* thm \<open>{start2 \<Rightarrow> $x1=$x2}\<close> *)
 
-  hoare step1L: range 1 ~ \<emptyset> pre start2 post step1L = default
+  hoare' step1L: range 1 ~ \<emptyset> pre start2 post step1L = default
+    (* TODO: should be automatic *)
+    by auto
 
   have [hoare_invi]: "{step1L \<Rightarrow> $x1=$x2+2}"
     apply wp
     using start2_inv_def by auto
 
-  hoare step1LR: range \<emptyset> ~ 1 pre step1L post step1LR = default
+  hoare' step1LR: range \<emptyset> ~ 1 pre step1L post step1LR = default
+    (* TODO: should be automatic *)
+    by auto
+
 (* TODO: pretty_range should include the \<emptyset> *)
 
   have bla [hoare_invi]: "{step1LR \<Rightarrow> $x1=$x2}"
@@ -138,7 +143,9 @@ lemma True proof
     using \<open>{step1L \<Rightarrow> $x1=$x2+2}\<close> 
     by auto
 
-  hoare step2: range 2~2 pre step1LR post step2 = default
+  hoare' step2: range 2~2 pre step1LR post step2 = default
+    (* TODO: should be automatic *)
+    by auto
 
    (* hoare preserve bla: \<open>{step1LR \<Rightarrow> $x1=$x2}\<close> in step2  *)
 
@@ -150,10 +157,15 @@ lemma True proof
     using \<open>{step1LR \<Rightarrow> $x1=$x2}\<close>
     by simp
 
-  (* TODO: Use joint sample postcondition *)
-  hoare step3: range 3~3 pre step2 post step3 = default
+(* TODO: make global *)
+  have [simp]: "semantics [] = return_spmf"
+    by auto
 
-  (* TODO: show \<open>{step3 \<Rightarrow> $y1+1=$y2}\<close> *)
+  (* TODO: Use joint sample postcondition *)
+  hoare' step3: range 3~3 pre step2 post step3 = default
+    by auto
+
+(* TODO: show \<open>{step3 \<Rightarrow> $y1+1=$y2}\<close> *)
 
   from \<open>{step3 \<Rightarrow> $x1=$x2}\<close> \<open>{step3 \<Rightarrow> $z1=$z2}\<close>
   have [hoare_invi]: "{step3 \<Rightarrow> $x1*$z1 = $x2*$z2}"
